Splinter/Journal/MarshalledJournal.i.dfy
@@ -9,24 +9,33 @@ module MarshalledJournal {
   import opened MsgHistoryMod
   import opened LSNMod
   import opened Sequences
-  import opened JournalLabels
+  import JournalLabels
   import opened Maps
   import LinkedJournal
 
-  type Block(!new, ==)
-  function Parse<T>(block: Block) : T
-  function Marshal<T>(t: T) : Block
-  lemma ParseAxiom<T>(t: T)
-    ensures Parse(Marshal(t)) == t
+  datatype JournalSB = JournalSB(
+    boundaryLSN: LSN,
+    freshestRec: Pointer)
 
-  type Address = LinkedJournal.Address
-  type Pointer = LinkedJournal.Pointer
-  type Disk = map<Address, Block>
+  datatype JournalImage = JournalImage(
+    superblock: JournalSB,
+    blockDiskView: Disk)
+
+  // TODO(jonh): appeal to parent lbl
+  datatype TransitionLabel =
+      ReadForRecoveryLabel(messages: MsgHistory)
+    | FreezeForCommitLabel(frozenJournal: MsgHistory, journalImage: JournalImage)
+    | QueryEndLsnLabel(endLsn: LSN)
+    | PutLabel(messages: MsgHistory)
+    | DiscardOldLabel(startLsn: LSN, requireEnd: LSN)
+      // TODO(jonh): requireEnd is an enabling-condition check to enforce
+      // MapIsFresh in CommitComplete. I don't think it's actually necessary,
+      // but removing it broke the CoordinationSystemRefinement proof and I
+      // couldn't fix it in five minutes.
+    | InternalLabel()
 
   datatype Variables = Variables(
-    disk: Disk,
-    freshestRec: Pointer,
-    boundaryLSN: LSN,
+    journalImage: JournalImage,
     unmarshalledTail: MsgHistory)
 
   function MarshalDisk(typed: map<Address, LinkedJournal.JournalRecord>) : Disk
@@ -42,11 +51,52 @@ module MarshalledJournal {
     && typed.truncatedJournal.diskView.boundaryLSN == v.boundaryLSN
   }
 
-  predicate Init(v: Variables, tj: LinkedJournal.TruncatedJournal)
+  function JournalImageI() : LinkedJournal.TruncatedJournal
+  {
+    true
+  }
+
+  function I(v: Variables) : LinkedJournal.Variables {
+    LinkedJournal.Variables(v.journalImage.I(), v.unmarshalledTail)
+  }
+
+  predicate Init(v: Variables, journalImage: JournalImage)
   {
     (exists t ::
       && TypeProvidesModel(v, t)
       && LinkedJournal.Init(t, tj)
+      && v.disk == journalImage.blockDiskView
+      && v.boundaryLSN == journalImage.superblock.boundaryLSN
+      && v.freshestRec == journalImage.superblock.pointer
+//      && v.unmarshalledTail.IsEmpty() // Implied by LinkedJournal.Init && TypeProvidesModel.
+    )
+  }
+
+  predicate FreezeForCommit(v: Variables, v': Variables, lbl: TransitionLabel, keepReceiptLines: nat)
+  {
+    (exists t, t' ::
+      // Connection up a layer
+      && TypeProvidesModel(v, t)
+      && TypeProvidesModel(v', t')
+      && LinkedJournal.Next(t, t', lbl)
+
+      // Have a tight model of the disk that's rooted where the SB points.
+      && var fr := journalImage.superblock.freshestRec;
+      && lbl.journalImage.blockDiskView.WF()
+      && lbl.journalImage.blockDiskView.IsSubDisk(v.disk)
+      && lbl.journalImage.blockDiskView.IsNondanglingPointer(fr)
+      && lbl.journalImage.blockDiskView.Tight()
+
+      // Start where the v journal starts
+      && lbl.journalImage.superblock.boundaryLSN == v.boundaryLSN
+
+      // End at a block that matches the end we promised in the (abstract ghosty) frozenJournal
+      && (if lbl.frozenJournal.IsEmpty()
+          then fr.None?
+          else
+            && fr.Some?
+            && t.diskView[fr.value].messageSeq.seqEnd == lbl.frozenJournal.seqEnd
+         )
     )
   }
 
@@ -54,12 +104,13 @@ module MarshalledJournal {
     && (exists typed :: TypeProvidesModel(v, typed))
   }
 
-  predicate Next(v: Variables, v': Variables, lbl: TransitionLabel)
+  predicate Next(v: Variables, v': Variables, lbl: TransitionLabel, journalImage: JournalImage)
   {
     (exists t, t' ::
       && TypeProvidesModel(v, t)
       && TypeProvidesModel(v', t')
       && LinkedJournal.Next(t, t', lbl)
+      && AdditionalStupidConstraint(v, v', t, lbl, journalImage)
     )
   }
 }
